v2/examples/counter/lakefile.lean
@@ -10,14 +10,6 @@ lean_lib Counter where
   srcDir := "src"
   roots := #[`Counter]
 
-lean_lib CounterDSL where
-  srcDir := "src"
-  roots := #[`CounterDSL]
-
-lean_lib CounterProofs where
-  srcDir := "test"
-  roots := #[`CounterProofs]
-
 lean_lib CounterTheorem where
   srcDir := "test"
   roots := #[`CounterTheorem]
