v2/TODO.md
@@ -1,0 +1,1 @@
+[ ] evaluate if we should add Optional<Address> to replace Address 0
